MiniKernel/LevelProofs.lean
@@ -1,0 +1,474 @@
+import MiniKernel.Types
+
+/-!
+This module explores the level inequality procedure and proves it correct but incomplete.
+
+Because the function in `Kernel.lean` is implemented as a partial function, and
+to avoid cluttering that file with the setup to make the termination proof go through,
+we have a copy of that function here.
+-/
+
+def Level.substLevel (l : Level) (f : Name → Level) : Level :=
+  match l with
+  | .param n => f n
+  | .zero => .zero
+  | .succ l' => .succ (l'.substLevel f)
+  | .max l1 l2 => .max (l1.substLevel f) (l2.substLevel f)
+  | .imax l1 l2 => .imax (l1.substLevel f) (l2.substLevel f)
+
+def Level.substOneLevel (l : Level) (n : Name) (l' : Level) : Level :=
+  l.substLevel fun m => if m == n then l' else .param m
+
+
+/--
+Smart constructor that ensures the invariant that the rhs of `imax` is always a parameter.
+-/
+def Level.mkIMax (l1 l2 : Level) : Level :=
+  match l2 with
+  | .zero =>        .zero
+  | .succ _ =>      .max l1 l2
+  | .max l21 l22 => .max (l1.mkIMax l21) (l1.mkIMax l22)
+  | .imax l21 l22 =>.mkIMax (l1.max l21) l22
+  | .param _  =>    .imax l1 l2
+
+/--
+Simplification ensures the invariant that the rhs of an `imax` is always a parameter.
+-/
+def Level.simplify : Level → Level
+  | .zero => .zero
+  | .succ l => .succ l.simplify
+  | .max l1 l2 => .max l1.simplify l2.simplify
+  | .imax l1 l2 => .mkIMax l1.simplify l2.simplify
+  | .param n => .param n
+
+/--
+Restricted simplification; only eliminates IMax, but does not duplicate terms.
+(Necessary to prove well-foundedness of the `le` implications)
+-/
+def Level.elimIMax : Level → Level
+  | .zero => .zero
+  | .succ l => .succ l.elimIMax
+  | .max l1 l2 => .max l1.elimIMax l2.elimIMax
+  | .imax _ .zero => .zero
+  | .imax l1 (.succ l2) => .max l1.elimIMax (.succ l2.elimIMax)
+  | .imax l1 l2 => .imax l1.elimIMax l2.elimIMax
+  | .param n => .param n
+
+def Level.byCases (p : Name) (l1 l2 : Level) (k : (l1 l2 : Level) → Bool) : Bool :=
+  k (l1.substOneLevel p Level.zero).elimIMax (l2.substOneLevel p Level.zero).elimIMax &&
+  k (l1.substOneLevel p (Level.param p).succ).elimIMax (l2.substOneLevel p (Level.param p).succ).elimIMax
+
+def Level.countIMax : Level → Nat
+  | .zero => 0
+  | .succ l => l.countIMax
+  | .max l1 l2 => l1.countIMax + l2.countIMax
+  | .imax l1 l2 => l1.countIMax + l2.countIMax + 1
+  | .param _ => 0
+
+theorem Level.countIMax_elimIMax (l : Level) : l.elimIMax.countIMax ≤ l.countIMax := by
+  fun_induction Level.elimIMax <;> grind [countIMax]
+grind_pattern Level.countIMax_elimIMax => l.elimIMax.countIMax
+
+theorem Level.countIMax_substOneLevel (l1 l2 : Level) (h : l2.countIMax = 0) :
+  (l1.substOneLevel p l2).countIMax ≤ l1.countIMax := by
+  unfold substOneLevel
+  fun_induction substLevel <;> grind [countIMax]
+grind_pattern Level.countIMax_substOneLevel => (l1.substOneLevel p l2).countIMax
+
+@[simp, grind =] theorem Level.substOneLevel_imax (l1 l2 l3 : Level) :
+  (l1.imax l2).substOneLevel p l3 = .imax (l1.substOneLevel p l3) (l2.substOneLevel p l3) := rfl
+@[simp, grind =] theorem Level.substOneLevel_param_self : (param p).substOneLevel p  l = l := by
+  simp [substOneLevel, substLevel]
+
+/-- Variant of `Level.byCases'` with a stronger type that helps with termination checking -/
+def Level.byCases' (p : Name) (l1 l2 : Level)
+  (k : (l1' l2' : Level) →
+    ((∃ l, l1 = .imax l (.param p) ∨ l2 = .imax l (.param p)) → l1'.countIMax + l2'.countIMax < l1.countIMax + l2.countIMax) → Bool) : Bool :=
+  k (l1.substOneLevel p Level.zero).elimIMax (l2.substOneLevel p Level.zero).elimIMax ?p1 &&
+  k (l1.substOneLevel p (Level.param p).succ).elimIMax (l2.substOneLevel p (Level.param p).succ).elimIMax ?p2
+where finally
+  · grind [elimIMax, countIMax]
+  · grind [elimIMax, countIMax]
+
+@[wf_preprocess] theorem Level.byCases_eq_byCases' :
+  Level.byCases p l1 l2 k = Level.byCases' p l1 l2 (fun l1' l2' _h => k l1' l2') := rfl
+
+-- Implementation inspired by https://ammkrn.github.io/type_checking_in_lean4/levels.html
+def Level.le (l1 l2 : Level) (balance : Int := 0) : Bool :=
+  match _ : l1, _ : l2, decide (0 ≤ balance) with
+  | .succ l1', l2, _ => Level.le l1' l2 (balance - 1)
+  | l1, .succ l2', _ => Level.le l1 l2' (balance + 1)
+  | .max l1a l1b, l2, _ =>
+    Level.le l1a l2 balance && Level.le l1b l2 balance
+  | .param n, .param m, _ => n == m && balance >= 0
+  | .imax _ (.param p), _, _ | _, .imax _ (.param p), _ =>
+    Level.byCases p l1 l2 (fun l1' l2' => Level.le l1' l2' balance)
+  | .imax _ _, _, _ | _, .imax _ _, _  => false -- unreachable by the simplification invariant
+  | param _, .max l2a l2b, _ | zero, .max l2a l2b, _  =>
+    Level.le l1 l2a balance || Level.le l1 l2b balance
+  | .zero, _, true => true
+  | .zero, .param _, false => false
+  | _, .zero, false => false
+  | .param _, .zero, _ => false
+termination_by (l1.countIMax + l2.countIMax, sizeOf l1 + sizeOf l2)
+decreasing_by
+  all_goals try solve
+    | apply Prod.Lex.right'
+      · grind [countIMax]
+      · grind [Level.succ.sizeOf_spec, Level.max.sizeOf_spec]
+    | apply Prod.Lex.left
+      subst l1 l2
+      grind [countIMax]
+
+/--
+The simplified form for levels: The rhs of an `imax` is always a parameter.
+-/
+@[grind] inductive Level.NF : Level → Prop
+  | zero : Level.NF .zero
+  | succ : Level.NF l → Level.NF (.succ l)
+  | max : Level.NF l1 → Level.NF l2 → Level.NF (.max l1 l2)
+  | imax : Level.NF l1 → Level.NF (.imax l1 (.param u))
+  | param : Level.NF (.param n)
+
+@[grind .] theorem Level.NF.mkIMax (h1 : Level.NF l1) (h2 : Level.NF l2) : Level.NF (.mkIMax l1 l2) := by
+  fun_induction Level.mkIMax <;> grind
+
+@[grind .] theorem Level.NF.simplify : Level.NF (simplify l) := by
+  fun_induction Level.simplify <;> grind
+
+
+def Level.eval (l : Level) (ctx : Name → Nat) : Nat :=
+  match l with
+  | .zero => 0
+  | .succ l' => l'.eval ctx + 1
+  | .max l1 l2 => Nat.max (l1.eval ctx) (l2.eval ctx)
+  | .imax l1 l2 => if (l2.eval ctx) = 0 then 0 else Nat.max (l1.eval ctx) (l2.eval ctx)
+  | .param n => ctx n
+
+theorem Level.eval_mono (ctx1 ctx2 : Name → Nat) (l : Level)
+  (hmono : ∀ n, ctx1 n ≤ ctx2 n) : l.eval ctx1 ≤ l.eval ctx2 := by
+  fun_induction Level.eval l ctx1 <;> grind [eval]
+
+@[grind =] theorem Level.mkIMax_correct (ctx : Name → Nat) (l1 l2 : Level): (mkIMax l1 l2).eval ctx = (Level.imax l1 l2).eval ctx := by
+  fun_induction mkIMax<;> try grind [Level.eval]
+
+@[simp] theorem Level.elimIMax_correct (ctx : Name → Nat) (l : Level): l.elimIMax.eval ctx = l.eval ctx := by
+  fun_induction Level.elimIMax <;> grind [Level.eval]
+
+@[simp] theorem Level.simplify_correct (ctx : Name → Nat) (l : Level): l.simplify.eval ctx = l.eval ctx := by
+  fun_induction Level.simplify <;> grind [Level.eval]
+
+theorem Level.substOneLevel_eval' {ctx ctx' p} (l1 l2 : Level)
+  (h : l2.eval ctx' = ctx p)
+  (h2 : ∀ p', p ≠ p' → ctx' p' = ctx p') :
+  (l1.substOneLevel p l2).eval ctx' = l1.eval ctx := by
+  unfold substOneLevel
+  fun_induction substLevel <;> grind [Level.eval]
+
+theorem Level.substOneLevel_eval (l1 l2 : Level) (h : l2.eval ctx = ctx p):
+  (l1.substOneLevel p l2).eval ctx = l1.eval ctx :=
+  Level.substOneLevel_eval' _ _ h (by grind)
+
+/-- Correctness of `Level.le` -/
+theorem Level.le_correct (ctx : Name → Nat) (l1 l2 : Level) balance : l1.le l2 balance = true → l1.eval ctx ≤ l2.eval ctx + balance := by
+  fun_induction Level.le l1 l2 balance generalizing ctx <;> try grind [Level.eval]
+  case case5 l2 balance l1 p _ ih =>
+    match h : ctx p with
+    | .zero =>
+      unfold byCases
+      specialize ih ((l1.imax (param p)).substOneLevel p .zero).elimIMax
+                    (l2.substOneLevel p .zero).elimIMax
+                    (fun _ => by grind [countIMax, elimIMax])
+                    ctx
+      simp [elimIMax] at ih
+      intro hle
+      specialize ih (by simp [elimIMax] at hle; grind)
+      simp [eval] at ih
+      rw [Level.substOneLevel_eval] at ih
+      case h => simp [h, eval]
+      simp [eval, h]
+      assumption
+    | .succ n =>
+      unfold byCases
+      specialize ih ((l1.imax (param p)).substOneLevel p ((Level.param p).succ)).elimIMax
+                    (l2.substOneLevel p ((Level.param p).succ)).elimIMax
+                    (fun _ => by grind [countIMax, elimIMax])
+                    (fun p' => if p' = p then n else ctx p')
+      simp [elimIMax] at ih
+      intro hle
+      specialize ih (by simp [elimIMax] at hle; grind)
+      simp [eval] at ih
+      rw [Level.substOneLevel_eval' (ctx := ctx)] at ih
+      case h => simp [h, eval]
+      case h2 => grind
+      rw [Level.substOneLevel_eval' (ctx := ctx)] at ih
+      case h => simp [h, eval]
+      case h2 => grind
+      simp [eval, h]
+      assumption
+  case case6 l1 balance l2 p _ _ _ ih =>
+    match h : ctx p with
+    | .zero =>
+      unfold byCases
+      specialize ih (l1.substOneLevel p .zero).elimIMax
+                    ((l2.imax (param p)).substOneLevel p .zero).elimIMax
+                    (fun _ => by grind [countIMax, elimIMax])
+                    ctx
+      simp [elimIMax] at ih
+      intro hle
+      specialize ih (by simp [elimIMax] at hle; grind)
+      simp [eval] at ih
+      rw [Level.substOneLevel_eval] at ih
+      case h => simp [h, eval]
+      simp [eval, h]
+      assumption
+    | .succ n =>
+      unfold byCases
+      specialize ih (l1.substOneLevel p ((Level.param p).succ)).elimIMax
+                   ((l2.imax (param p)).substOneLevel p ((Level.param p).succ)).elimIMax
+                    (fun _ => by grind [countIMax, elimIMax])
+                    (fun p' => if p' = p then n else ctx p')
+      simp [elimIMax] at ih
+      intro hle
+      specialize ih (by simp [elimIMax] at hle; grind)
+      simp [eval] at ih
+      rw [Level.substOneLevel_eval' (ctx := ctx)] at ih
+      case h => simp [h, eval]
+      case h2 => grind
+      rw [Level.substOneLevel_eval' (ctx := ctx)] at ih
+      case h => simp [h, eval]
+      case h2 => grind
+      simp [eval, h]
+      assumption
+
+
+/-- Incompleteness of `Level.le` -/
+theorem Level.le_incompleteness (p : Name) :
+  let l1 := (Level.param p).succ
+  let l2 := (Level.zero.succ).max (.imax ((Level.param p).succ) (.param p))
+  (∀ ctx, l1.eval ctx ≤ l2.eval ctx) ∧ l1.le l2 = false := by
+  constructor
+  · intro ctx
+    simp [eval]
+    grind
+  · simp [le, byCases, elimIMax]
+
+/-!
+The rest of the file are lemmas created while investigating completeness.
+-/
+
+
+theorem Level.forall_zero_le_eval (balance : Int) (l : Level) :
+  (∀ ctx, 0 ≤ l.eval ctx + balance) ↔ 0 ≤ l.eval (fun _ => 0) + balance:= by
+  constructor
+  · intro h; apply h
+  · intro h0 ctx
+    have := Level.eval_mono (fun _ => 0) ctx l (by grind)
+    grind
+
+def Option.imax (o1 o2 : Option Nat) : Option Nat :=
+  match o1, o2 with
+  | none, none => none
+  | _, none => none
+  | none, some n => some n
+  | some n1, some n2 => some (Nat.max n1 n2)
+
+def Level.coeff (l : Level) (p : Name) : Option Nat :=
+  match l with
+  | .zero => none
+  | .succ l' => .succ <$> coeff l' p
+  | .max l1 l2 => Max.max (coeff l1 p) (coeff l2 p)
+  | .imax l1 (.param n) => if n = p then Max.max (coeff l1 p) (some 0) else none
+  | .imax _ _ => none -- unreachable due to NF
+  | .param n => if n = p then some 0 else none
+
+theorem Level.coeff_le_eval_none (n : Nat) (l : Level) (p : Name)
+  (hwf : l.NF) (h : l.coeff p = none) : l.eval (fun p' => if p' = p then n else 0) = l.eval (fun _ => 0) := by
+  induction hwf generalizing n <;> simp_all only [coeff] <;> simp_all [eval]
+
+theorem Level.coeff_some_eval (l : Level) (p : Name) (hwf : l.NF) (h : l.coeff p = some c) :
+    ∃ n, ∀ m > n, l.eval (fun p' => if p' = p then m else 0) = c + m := by
+  induction hwf generalizing c <;> simp_all only [coeff, eval] <;> try grind [coeff, eval, Functor.map]
+  case succ l hwf ih =>
+    revert ih h; cases l.coeff p <;> intro ih h
+    · contradiction
+    · simp at h; subst c
+      obtain ⟨n, ih⟩ := ih rfl
+      exists n
+      intro m hm
+      grind
+  case max l1 l2 hwf1 hwf2 ih1 ih2 =>
+    revert ih1 ih2 h; cases hc1 : l1.coeff p <;> cases hc2 : l2.coeff p <;> intro ih1 ih2 h <;> simp at h
+    · subst c
+      clear ih1
+      obtain ⟨n2, ih2⟩ := ih2 rfl
+      exists Max.max (l1.eval (fun _ => 0)) n2
+      intro m hm
+      rw [Level.coeff_le_eval_none _ l1 p hwf1 hc1]
+      specialize ih2 m (by grind)
+      grind
+    · subst c
+      clear ih2
+      obtain ⟨n1, ih1⟩ := ih1 rfl
+      exists Max.max n1 (l2.eval (fun _ => 0))
+      intro m hm
+      rw [Level.coeff_le_eval_none _ l2 p hwf2 hc2]
+      specialize ih1 m (by grind)
+      grind
+    · subst c
+      obtain ⟨n1, ih1⟩ := ih1 rfl
+      obtain ⟨n2, ih2⟩ := ih2 rfl
+      exists Max.max n1 n2
+      intro m hm
+      specialize ih1 m (by grind)
+      specialize ih2 m (by grind)
+      grind
+  case imax l1 p' hwf1 ih1 =>
+    by_cases hp : p' = p
+    · simp [hp] at *
+      skip
+      revert ih1 h; cases h1 : l1.coeff p <;> intro ih1 h <;> simp at h <;> subst h
+      case pos.none =>
+        exists l1.eval (fun _ => 0)
+        intro m hm
+        rw [Level.coeff_le_eval_none _ l1 p hwf1 h1]
+        grind
+      case pos.some c =>
+        simp_all
+        obtain ⟨n1, ih1⟩ := ih1
+        exists n1
+        intro m hm
+        specialize ih1 m (by grind)
+        grind
+    · simp [hp] at *
+  case param n =>
+    simp at h
+    exists 0
+    grind
+
+theorem Level.coeff_le_eval_some (l : Level) (p : Name) (ctx : Name → Nat)
+  (hwf : l.NF) (h : l.coeff p = some n) (hp : 0 < ctx p) : n + ctx p ≤ l.eval ctx := by
+  induction hwf generalizing n <;> simp_all only [coeff] <;> try grind [coeff, eval, Functor.map]
+  case succ =>
+    simp_all [Functor.map, eval]; grind
+  case max l1 l2 hl1 hl2 ih1 ih2 =>
+    simp_all [eval]
+    revert ih1 ih2 h
+    cases l1.coeff p <;> cases l2.coeff p <;> grind
+  case imax l1 p' hl1 ih1 =>
+    simp_all [eval]
+    revert ih1 h
+    cases l1.coeff p <;> by_cases p' = p <;> grind
+
+theorem Level.forall_param_le_eval (balance : Int) (l : Level) (p : Name) (hwf : l.NF) :
+  (∀ ctx, ctx p ≤ l.eval ctx + balance) ↔
+  (0 ≤ l.eval (fun _ => 0) + balance ∧ ∃ n, l.coeff p = some n ∧ 0 ≤ n + balance) := by
+  cases h : l.coeff p
+  case none =>
+    constructor
+    · intro h
+      exfalso
+      specialize h (fun p' => if p' = p then Int.natAbs balance + l.eval (fun _ => 0) + 1 else 0)
+      have := Level.coeff_le_eval_none (Int.natAbs balance + l.eval (fun _ => 0) + 1) l p hwf ‹_›
+      simp_all
+      grind
+    · simp
+  case some n =>
+    constructor
+    · intro h
+      constructor
+      · apply h
+      · simp
+        obtain ⟨k, hk⟩ := Level.coeff_some_eval l p hwf ‹_›
+        specialize hk (k+1) (by grind)
+        specialize h (fun p' => if p' = p then k + 1 else 0)
+        rw [hk] at h; clear hk
+        grind
+    · intro ⟨h1,h2⟩ ctx
+      by_cases h0 : ctx p = 0
+      · simp [h0] at *
+        have := Level.eval_mono (fun _ => 0) ctx l (by grind)
+        grind
+      · have := Level.coeff_le_eval_some l p ctx hwf ‹_›
+        obtain ⟨_, heq, h2⟩ := h2
+        simp at heq; subst heq
+        grind
+
+theorem max_is_wrong (p : Name) :
+  let l1 := Level.zero.succ
+  let l2 := .imax ((Level.param p).succ) (.param p)
+  let balance : Int := -1
+  let ctx1 := fun n => if n = p then 2 else 0
+  let ctx2 := fun n => if n = p then 0 else 0
+  (l1.NF) ∧ (l2.NF) ∧
+  (∀ ctx, ctx p ≤ (l1.max l2).eval ctx + balance) ∧
+  (¬ ctx1 p ≤ l1.eval ctx1 + balance) ∧ (¬ ctx2 p ≤ l2.eval ctx2 + balance) := by
+  constructor
+  · constructor; constructor
+  constructor
+  · constructor; constructor; constructor
+  constructor
+  · intro ctx
+    simp [Level.eval]
+    grind
+  · constructor
+    · simp [Level.eval]
+    · simp [Level.eval]
+
+
+theorem Level.forall_param_le_eval' (balance : Int) (l : Level) (p : Name) :
+  (∀ ctx, ctx p ≤ l.eval ctx + balance) ↔
+  (∀ n, n ≤ l.eval (fun n' => if n' = p then n else 0) + balance) := by
+  constructor
+  · intro h n
+    specialize h (fun n' => if n' = p then n else 0)
+    grind
+  · intro h ctx
+    specialize h (ctx p)
+    have := Level.eval_mono (fun n' => if n' = p then ctx p else 0) ctx l (by grind)
+    simp_all
+    grind
+
+/-
+theorem Level.le_complete (ctx : Name → Nat) (l1 l2 : Level) (balance : Int) :
+    (∀ ctx, l1.eval ctx ≤ l2.eval ctx + balance) → l1.le l2 balance = true := by
+  intro hle
+  fun_induction Level.le l1 l2 balance <;> try grind [Level.eval]
+  case case4 balance p1 p2 => -- param case
+    by_cases p2 = p1
+    · subst p2
+      specialize hle (fun _ => 0)
+      simp_all [eval]
+    · exfalso
+      specialize hle (fun p' => if p' = p1 then Int.natAbs balance + 1 else 0)
+      grind [eval]
+  case case5 => -- byCases case
+    sorry
+  case case6 => -- byCases case 2
+    sorry
+  case case7 => -- unreachable case due to NF
+    sorry
+  case case8 => -- unreachable case due to NF
+    sorry
+  case case9 => -- param le max
+    simp only [Bool.or_eq_true]
+    simp [eval.eq_5] at *
+    sorry
+    -- This is where the proof falls apart
+  case case10 => -- zero le max
+    simp only [Bool.or_eq_true]
+    simp [eval.eq_1, Level.forall_zero_le_eval] at *
+    grind [eval.eq_3]
+  case case12 =>
+    simp_all [eval]
+    specialize hle (fun _ => 0)
+    grind
+  case case13 =>
+    simp_all [eval]
+    specialize hle (fun _ => 0)
+    grind
+  case case14 balance _ _ =>
+    simp_all [eval]
+    specialize hle (fun _ => Int.natAbs balance + 1)
+    grind
+-/
